testdata/wild/let-shadowed-by-descendant-field-in-struct/let-shadowed-by-descendant-field-in-struct.cue
@@ -1,0 +1,6 @@
+package repro
+out: {
+	let x = 1
+	lst: [{x: 2}]
+	got: x
+}
