testdata/wild/let-shadowed-by-field-in-def-body/let-shadowed-by-field-in-def-body.cue
@@ -1,0 +1,6 @@
+package repro
+let x = 1
+#d: {
+	x: 2
+}
+out: x
