testdata/wild/let-shadowed-by-nested-field/let-shadowed-by-nested-field.cue
@@ -1,0 +1,6 @@
+package repro
+let x = 1
+out: {
+	x: 2
+	got: x
+}
